Regex/Lemmas/Bounds.lean
@@ -6,60 +6,7 @@ version of `star_terminates` -/
 namespace Regex
 
 variable {α : Type u} [deq : DecidableEq α] {r : Regex α} {w : List α}
-  {s : ℕ} {cap : Captures} {term : r.Terminates w s cap}
-
-def decreasingStrongRec {n : ℕ} {motive : (m : ℕ) → m ≤ n → Sort u}
-    (ind : ∀ m, (mn : m ≤ n) →
-      (∀ k, (kn : k ≤ n) → (km : k > m) → motive k kn) →
-      motive m mn)
-    (m : ℕ) (mn : m ≤ n)
-    : motive m mn :=
-  ind m mn fun k kn _ ↦ decreasingStrongRec ind k kn
-
-/-- The property that all matches that end in bounds. -/
-def EndsInBounds (r : Regex α) (w : List α) (s : ℕ) (cap : Captures)
-    (term : r.Terminates w s cap) :=
-    ∀ {mat},
-      mat ∈ r.matchPartial w s cap term → mat.1 ≤ w.length
-
---/-- If a start index that is at most `w.length` is supplied (i.e. is in bounds),
---then all matches end in bounds. -/
---theorem matchPartial_inBounds_le (hs : s ≤ w.length) : r.EndsInBounds w s cap term := by
---  revert term
---  induction s, hs using decreasingStrongRec generalizing cap with | ind s slt ind =>
---    intro term
---    induction r with
---    | bot => simp [matchPartial_bot] at mem
---    | empty => simp [matchPartial_empty, Prod.eq_iff_fst_eq_snd_eq] at ind mem; simp [mem, slt]
---    | unit _ =>
---      simp only [matchPartial_unit, List.getElem?_eq_some_iff, List.mem_ite_nil_right, List.mem_cons,
---        List.not_mem_nil, or_false] at mem
---      rcases mem with ⟨⟨lt, _⟩, mateq⟩
---      simp [mateq, lt]
---    | concat q r qind rind =>
---      simp [matchPartial_concat] at ind mem
---      rcases mem with ⟨s', cap', qmem, rmem⟩
---      specialize qind hs qmem
---      simp only at qind
---      exact rind qind rmem
---    | or q r qind rind =>
---      simp only [matchPartial_or, List.mem_append] at mem
---      exact Or.casesOn mem (fun mem ↦ qind hs mem) (fun mem ↦ rind hs mem)
---    | filterEmpty _ r rind =>
---      simp only [matchPartial_filterEmpty, ge_iff_le, eq_iff_iff, Bool.decide_iff_dist,
---        Bool.decide_eq_true, List.mem_filter, beq_iff_eq] at mem
---      exact rind hs mem.1
---    | star t r rind =>
---      simp only [matchPartial_star] at mem
---      cases t
---      case greedy | lazy =>
---        simp [matchPartial_or, matchPartial_concat, matchPartial_filterEmpty,
---          matchPartial_empty] at mem
---        try rw [or_comm (a := mat = _), or_assoc] at mem
---        rcases mem with mem | ⟨s', cap', mem', _⟩ | eq
---        · exact rind hs mem.1
---        · specialize rind hs mem'.1; simp only at rind; exact _
---        · simp [eq]
+  {s : ℕ} {cap : Captures}
 
 /-- If a start index that is `w.length` or out of bounds is supplied,
 there are no positive-length matches. -/
@@ -125,6 +72,81 @@ theorem matchPartial_outOfBounds_eq {term : r.Terminates w s cap}
         List.drop_eq_nil_iff] at h
       rwa [← Nat.sub_eq_zero_iff_le] at h
 
+/-- The property that matches with this regex always end in bounds
+(i.e. at a position ≤ `w.length`) -/
+def EndInBounds (r : Regex α) :=
+  ∀ w s, s ≤ w.length → ∀ cap (term : r.Terminates w s cap) mat,
+    mat ∈ r.matchPartial w s cap term → mat.1 ≤ w.length
+
+/-- Stars end in bounds. Must be proved separately due to star recursion. -/
+theorem endInBounds_star {t : StarType} (hr : r.EndInBounds)
+    : [/⟨r⟩*‹t›/].EndInBounds := by
+  intro w s sle cap term mat mem
+  induction s, sle using decreasingStrongRec generalizing r cap mat with | ind s sle ind =>
+  simp only [matchPartial_star] at mem
+  cases t
+  case greedy | lazy =>
+    simp only [matchPartial_or, matchPartial_filterEmpty, ge_iff_le, eq_iff_iff, iff_true,
+      matchPartial_concat, Bool.false_eq_true, iff_false, not_le, matchPartial_empty,
+      List.append_assoc, List.mem_append, List.mem_filter, decide_eq_true_eq, List.mem_flatten,
+      List.mem_pmap, Prod.exists, ↓existsAndEq, true_and, List.mem_cons, List.not_mem_nil,
+      or_false] at mem
+    try rw [or_comm (a := mat = _), or_assoc] at mem
+    rcases mem with mem | ⟨s', cap', mem, stmem⟩ | eq
+    · exact (.trans mem.2 sle)
+    · exact ind s' (hr _ _ sle _ _ _ mem.1) mem.2 hr _ _ _ stmem
+    · simp [eq, sle]
+
+/-- If a start index that is at most `w.length` is supplied (i.e. is in bounds),
+then all matches end in bounds. -/
+theorem endInBounds : r.EndInBounds := by
+  intro w s sle cap term mat mem
+  induction r generalizing w s cap mat with
+  | bot => simp [matchPartial_bot] at mem
+  | empty => simp [matchPartial_empty, Prod.eq_iff_fst_eq_snd_eq] at mem; simp [mem, sle]
+  | unit _ =>
+    simp only [matchPartial_unit, List.getElem?_eq_some_iff, List.mem_ite_nil_right, List.mem_cons,
+      List.not_mem_nil, or_false] at mem
+    rcases mem with ⟨⟨lt, _⟩, mateq⟩
+    simp [mateq, lt]
+  | concat q r qind rind =>
+    simp only [matchPartial_concat, List.mem_flatten, List.mem_pmap, Prod.exists, ↓existsAndEq,
+      true_and] at mem
+    rcases mem with ⟨s', cap', qmem, rmem⟩
+    specialize qind _ _ sle _ _ _ qmem
+    simp only at qind
+    exact rind _ _ qind _ _ _ rmem
+  | or q r qind rind =>
+    simp only [matchPartial_or, List.mem_append] at mem
+    exact Or.casesOn mem (fun mem ↦ qind _ _ sle _ _ _ mem) (fun mem ↦ rind _ _ sle _ _ _ mem)
+  | filterEmpty _ r rind =>
+    simp only [matchPartial_filterEmpty, ge_iff_le, eq_iff_iff, Bool.decide_iff_dist,
+      Bool.decide_eq_true, List.mem_filter, beq_iff_eq] at mem
+    exact rind _ _ sle _ _ _ mem.1
+  | star _ r rind =>
+    exact endInBounds_star rind _ _ sle _ _ _ mem
+  | start => simp [matchPartial_start] at mem; simp [mem]
+  | end' => simp [matchPartial_end'] at mem; simp [mem]
+  | capture _ r rind =>
+    simp only [matchPartial_capture, List.mem_map, Prod.eq_iff_fst_eq_snd_eq, Prod.exists,
+      ↓existsAndEq, true_and] at mem
+    rcases mem with ⟨cap', mem, _⟩
+    have le := rind _ _ sle _ _ _ mem
+    exact le
+  | backref d _ =>
+    simp only [matchPartial_backref, List.extract_eq_drop_take, List.length_take, List.length_drop,
+      add_tsub_cancel_left] at mem
+    split at mem
+    · split at mem <;> (simp at mem; try simp [mem, sle])
+    · split at mem <;> (expose_names; simp only [List.mem_cons, List.not_mem_nil, or_false] at mem)
+      apply_fun List.length at h
+      simp only [List.length_take, List.length_drop, Nat.min_assoc] at h
+      simp only [mem, ← h]
+      rw (occs := [3]) [← Nat.add_sub_cancel' sle]
+      refine Nat.add_le_add_left ?_ s
+      rw [min_comm, min_right_comm]
+      exact min_le_right _ _
+
 /-- `star t r` terminates if (but not only if)
 `r` terminates for every capture and for every position starting from here -/
 theorem star_terminates_of_forall {t : StarType}
@@ -141,5 +163,65 @@ theorem star_terminates_of_forall {t : StarType}
         (fun s' ge ↦ term s' (le_of_lt (Trans.trans lt ge))) rfl
     · have eq := matchPartial_outOfBounds_eq h mem
       exact (ne_of_lt lt eq).elim
+
+/-- The star type is interchangeable in a `Terminates` assertion -/
+theorem star_terminates_greedy_iff_lazy
+    : [/⟨r⟩*/].Terminates w s cap ↔ [/⟨r⟩*?/].Terminates w s cap := by
+  by_cases! sle : s ≤ w.length
+  focus induction s, sle using decreasingStrongRec generalizing cap
+  all_goals (
+    simp only [star_terminates']
+    rw [or_terminates_comm]
+    simp only [or_terminates, filterEmpty_terminates, concat_terminates,
+      matchPartial_filterEmpty, empty_terminates, true_and]
+    rw [iff_iff_eq]; congr; ext term
+    simp only [ge_iff_le, Bool.false_eq_true, eq_iff_iff, iff_false, not_le, List.mem_filter,
+      decide_eq_true_eq, and_imp, Prod.forall])
+  · rename_i s sle ind
+    constructor <;> (
+      intro left s' cap' mem lt
+      have bound := endInBounds _ _ sle _ _ _ mem
+      first | rw [ind _ bound lt] | rw [← ind _ bound lt]
+      exact left _ _ mem lt)
+  · constructor <;> (
+      intro left s' cap' mem lt
+      have bound := matchPartial_outOfBounds_eq (le_of_lt sle) mem
+      linarith)
+
+/-- The set of partial matches in the greedy and lazy versions of the same star
+are the same. -/
+theorem mem_matchPartial_star_greedy_iff_lazy {term : [/⟨r⟩*/].Terminates w s cap} {mat}
+    : mat ∈ [/⟨r⟩*/].matchPartial w s cap term ↔
+      mat ∈ [/⟨r⟩*?/].matchPartial w s cap (star_terminates_greedy_iff_lazy.mp term) := by
+  by_cases! sle : s ≤ w.length
+  focus induction s, sle using decreasingStrongRec generalizing cap
+  all_goals (
+    simp only [matchPartial_star]
+    rw [mem_matchPartial_or_comm]
+    simp only [matchPartial_or, matchPartial_empty, matchPartial_filterEmpty, ge_iff_le, eq_iff_iff,
+      iff_true, matchPartial_concat, Bool.false_eq_true, iff_false, not_le, List.cons_append,
+      List.nil_append, List.mem_cons, List.mem_append, List.mem_filter, decide_eq_true_eq,
+      List.mem_flatten, List.mem_pmap, Prod.exists, ↓existsAndEq, true_and]
+    rw [iff_iff_eq]; congr; ext s'
+  )
+  · rename_i s sle ind
+    constructor <;> (
+      rintro ⟨cap', mem, mem'⟩
+      have bound := endInBounds _ _ sle _ _ _ mem.1
+      first | rw [ind _ bound mem.2] at mem' | rw [← ind _ bound mem.2] at mem'
+      exact ⟨_, mem, mem'⟩)
+    generalize_proofs term' at mem'
+    exact star_terminates_greedy_iff_lazy.mpr term'
+  · constructor <;> (
+      rintro ⟨cap', mem, mem'⟩
+      have bound := matchPartial_outOfBounds_eq (le_of_lt sle) mem.1
+      linarith)
+
+/-- The set of partial matches in the greedy and lazy versions of the same star
+are the same. (lazy to greedy version, because a terminator is required) -/
+theorem mem_matchPartial_star_lazy_iff_greedy {term : [/⟨r⟩*?/].Terminates w s cap} {mat}
+    : mat ∈ [/⟨r⟩*?/].matchPartial w s cap term ↔
+      mat ∈ [/⟨r⟩*/].matchPartial w s cap (star_terminates_greedy_iff_lazy.mpr term) := by
+  rw [mem_matchPartial_star_greedy_iff_lazy]
 
 end Regex
