Regex/Regular.lean
@@ -1,5 +1,5 @@
-import Regex.Basic
-import Regex.Lemmas
+import Regex.Lemmas.Bounds
+import Regex.Lemmas.Monotone
 
 variable {α : Type u} [deq : DecidableEq α] {r : Regex α} {w : List α}
 
@@ -19,116 +19,159 @@ inductive classRegular : Regex α → Prop where
   | or q r : classRegular q → classRegular r → classRegular (or q r)
   | star t r : classRegular r → classRegular (star t r)
 
-section MatchPartialShrink
+section MatchPartialFree
 
-variable {s : Pos w} {cap : Captures w} {t : IccFrom s} {a : IccTo s} {b : IccFrom t}
+variable {s : ℕ} {cap : Captures}
 
 /-- A regex where `partialMatch` does not care about outside context
 like captures -/
 def MatchPartialFree (r : Regex α) :=
-  ∀ {w : List α} {s : Pos w} {cap : Captures w}
-      {term : r.Terminates w s cap} {s' : Pos w} {cap' : Captures w}
-      (mem : (s', cap') ∈ r.matchPartial w s cap term)
-      (wa : List α) (wb : List α) (cap₁ : Captures (wa ++ w.extract s.val s'.val ++ wb))
-      (term₁ : r.Terminates (wa ++ w.extract s.val s'.val ++ wb)
-        (s.recycle s s' (monotone mem) wa wb) cap₁),
-    ∃ cap₁', (s'.recycle s s' (le_refl _) wa wb, cap₁') ∈
-      r.matchPartial (wa ++ w.extract s.val s'.val ++ wb)
-        (s.recycle s s' (monotone mem) wa wb) cap₁ term₁
+  ∀ w s cap term mat, mat ∈ r.matchPartial w s cap term →
+  ∀ (wa wb : List α) cap₁ term₁,
+    ∃ cap₁', ((wa ++ w.extract s mat.1).length, cap₁') ∈
+      r.matchPartial (wa ++ w.extract s mat.1 ++ wb) wa.length cap₁ term₁
 
 theorem matchPartialFree_bot : MatchPartialFree ([/⊥/] : Regex α) := by
   simp [MatchPartialFree, matchPartial_bot]
 
 theorem matchPartialFree_empty : MatchPartialFree ([//] : Regex α) := by
-  simp only [MatchPartialFree, matchPartial_empty, List.mem_cons, Prod.mk.injEq, ← Icc.val_inj,
-    List.not_mem_nil, or_false, List.extract_eq_drop_take, Icc.recycle_val, tsub_self, add_zero,
-    Nat.add_eq_left, exists_eq_right, forall_and_index]
-  intro w s cap term t cap' teq
-  simp [teq]
+  simp [MatchPartialFree, matchPartial_empty]
 
 theorem matchPartialFree_unit (c : α) : MatchPartialFree [/c/] := by
-  simp only [MatchPartialFree, matchPartial_unit, List.mem_dite_nil_right, List.mem_cons,
-    Prod.mk.injEq, ← Icc.val_inj, Icc.succOfIndex_val, List.not_mem_nil, or_false, exists_and_left,
-    exists_prop, List.extract_eq_drop_take, List.append_assoc, Icc.recycle_val, tsub_self, add_zero,
-    Nat.add_left_cancel_iff, ↓existsAndEq, and_true, forall_and_index]
-  intro w s cap term s' cap' s'add wsc capeq wa wb cap₁ term₁
-  have ⟨lt, wsc⟩ := List.getElem?_eq_some_iff.mp wsc
-  have one : 1 ≤ w.length - s.val := by
-    by_contra!
-    rw [Nat.lt_one_iff, Nat.sub_eq_zero_iff_le] at this
-    exact not_le.mpr lt this
-  suffices (if s.val < w.length then w[s.val]? else wb[0]?) = some c by
-    simpa [s'add, List.getElem?_append]
-  rw [Nat.le_sub_iff_add_le' s.is_le, ← Nat.lt_iff_add_one_le] at one
-  simp [one, wsc]
+  simp only [MatchPartialFree, matchPartial_unit, List.mem_ite_nil_right, List.mem_cons,
+    List.not_mem_nil, or_false, List.extract_eq_drop_take, List.append_assoc, Prod.mk.injEq,
+    exists_and_left, ↓existsAndEq, and_true, and_imp,
+    forall_eq_apply_imp_iff, add_tsub_cancel_left]
+  intro w s cap term wsc wa wb cap₁ term₁
+  rw [List.getElem?_append_right (le_refl _), Nat.sub_self]
+  have ⟨slt, wsc⟩ := List.getElem?_eq_some_iff.mp wsc
+  rw [List.getElem?_append_left (by simp [slt])]
+  simp [wsc, Nat.add_one_le_of_lt (Nat.zero_lt_sub_of_lt slt)]
 
 theorem matchPartialFree_concat {q r : Regex α} (qf : q.MatchPartialFree)
     (rf : r.MatchPartialFree)
     : [/⟨q⟩ ⟨r⟩/].MatchPartialFree := by
   simp only [MatchPartialFree, matchPartial_concat, List.mem_flatten, List.mem_pmap, Prod.exists,
-    ↓existsAndEq, true_and, forall_exists_index] at ⊢
+    ↓existsAndEq, true_and, forall_exists_index, Prod.forall]
   intro w s cap term s'' cap'' s' cap' qmem rmem wa wb cap₁ term₁
-  -- Please excuse the massive ▸ spam ahead
-  have eaear := List.extract_append_extract_assoc_right (monotone qmem) (monotone rmem) wa wb
-  have rear := Icc.recycle_extract_append_right (le_refl s) (monotone qmem) (monotone rmem) wa wb
-  have eaeal := List.extract_append_extract_assoc_left (monotone qmem) (monotone rmem) wa wb
-  have real := Icc.recycle_extract_append_left (monotone qmem) (monotone rmem) (le_refl s'') wa wb
-  -- And the ▸s have gotten slow
-  have qf₁ := qf qmem wa (w.extract s'.val s''.val ++ wb)
-  simp only [rear] at qf₁
-  rw! (castMode := .all) [eaear] at qf₁
-  specialize qf₁ cap₁ (concat_terminates.mp term₁).1
-  have ⟨cap₁', qf₁⟩ := qf₁
-  simp only at qf₁
-  have rf₁ := rf rmem (wa ++ w.extract s.val s'.val) wb
-  simp only [real] at rf₁
-  rw! (castMode := .all) [eaeal] at rf₁
-  specialize rf₁ cap₁' (by
-    have term' := (concat_terminates.mp term₁).2 _ qf₁
-    simp only at term'
-    refine cast ?_ term'
-    congr 1
-    rw [Icc.recycle_extract_append_right (monotone qmem) (le_refl _),
-      Icc.recycle_extract_append_left (monotone qmem) (le_refl _)]
-    · simp only [List.extract_eq_drop_take, eqRec_eq_cast, cast_cast, cast_eq]
-    exact monotone rmem)
-  have ⟨cap₁'', rf₁⟩ := rf₁
-  simp only at rf₁
-  refine ⟨cap₁'', _, _, qf₁, cast ?_ rf₁⟩
-  congr 2
-  rw [Icc.recycle_extract_append_right (monotone qmem) (le_refl _),
-    Icc.recycle_extract_append_left (monotone qmem) (le_refl _)]
-  · simp only [List.extract_eq_drop_take, eqRec_eq_cast, cast_cast, cast_eq]
-  exact (monotone rmem)
+  specialize qf _ _ _ _ _ qmem wa (w.extract s' s'' ++ wb) cap₁
+  have qm := monotone _ _ _ _ _ qmem
+  have rm := monotone _ _ _ _ _ rmem
+  rw [List.extract_append_extract_assoc_right _ qm rm] at qf
+  have ⟨cap₁', qmem₁⟩ := qf (concat_terminates.mp term₁).1
+  specialize rf _ _ _ _ _ rmem (wa ++ w.extract s s') wb cap₁'
+  rw [List.extract_append_extract_assoc_left _ qm rm] at rf
+  have ⟨cap₁'', rmem₁⟩ := rf ((concat_terminates.mp term₁).2 _ qmem₁)
+  rw [List.append_assoc _ (w.extract s s'), List.extract_append_extract _ qm rm] at rmem₁
+  exact ⟨_, _, _, qmem₁, rmem₁⟩
 
 theorem matchPartialFree_or {q r : Regex α} (qf : q.MatchPartialFree)
     (rf : r.MatchPartialFree)
     : [/⟨q⟩ | ⟨r⟩/].MatchPartialFree := by
-  simp only [MatchPartialFree, matchPartial_or, List.mem_append]
+  simp only [MatchPartialFree, matchPartial_or, List.mem_append, Prod.forall]
   intro w s cap term s' cap' mem wa wb cap₁ term₁
   rcases mem with mem | mem
-  · have ⟨cap₁', mem'⟩ := qf mem wa wb cap₁ (or_terminates.mp term₁).1
+  · have ⟨cap₁', mem'⟩ := qf _ _ _ _ _ mem wa wb cap₁ (or_terminates.mp term₁).1
     exact ⟨cap₁', Or.inl mem'⟩
-  · have ⟨cap₁', mem'⟩ := rf mem wa wb cap₁ (or_terminates.mp term₁).2
+  · have ⟨cap₁', mem'⟩ := rf _ _ _ _ _ mem wa wb cap₁ (or_terminates.mp term₁).2
     exact ⟨cap₁', Or.inr mem'⟩
 
-theorem matchPartialFree_star_greedy {r : Regex α}
-    (rf : r.MatchPartialFree)
-    : [/⟨r⟩*/].MatchPartialFree := by
-  rw [MatchPartialFree]
-  simp only [matchPartial_star, star_terminates']
-  rw [← MatchPartialFree.eq_1]
-  refine matchPartialFree_or (matchPartialFree_or ?_ ?_) matchPartialFree_empty
-  ·
+theorem matchPartialFree_filterEmpty {e : Bool} {r : Regex α} (rf : r.MatchPartialFree)
+    : [/⟨r⟩ ‹e›ε/].MatchPartialFree := by
+  simp only [MatchPartialFree, matchPartial_filterEmpty, ge_iff_le, eq_iff_iff,
+    Bool.decide_iff_dist, Bool.decide_eq_true, List.mem_filter, beq_iff_eq,
+    and_imp, Prod.forall]
+  intro w s cap term s' cap' mem dec wa wb cap₁ term₁
+  have ⟨cap₁', mem₁⟩ := rf _ _ _ _ _ mem _ _ _ (filterEmpty_terminates.mp term₁)
+  refine ⟨cap₁', mem₁, ?_⟩
+  cases e with
+  | false =>
+    simp only [decide_eq_false_iff_not, not_le, List.extract_eq_drop_take, List.length_append,
+      List.length_take, List.length_drop, add_le_iff_nonpos_right, nonpos_iff_eq_zero,
+      Nat.min_eq_zero_iff, Bool.decide_or, Bool.or_eq_false_iff] at dec ⊢
+    refine ⟨fun eq ↦ not_lt.mpr (Nat.sub_eq_zero_iff_le.mp eq) dec, ?_⟩
+    by_contra!
+    rw [Nat.sub_eq_zero_iff_le] at this
+    have bound := matchPartial_outOfBounds_eq this mem
+    linarith
+  | true =>
+    simp only [decide_eq_true_eq, List.extract_eq_drop_take, List.length_append, List.length_take,
+      List.length_drop, add_le_iff_nonpos_right, nonpos_iff_eq_zero, Nat.min_eq_zero_iff,
+      Bool.decide_or, Bool.or_eq_true] at dec ⊢
+    have mono := monotone _ _ _ _ _ mem
+    have eq := le_antisymm mono dec
+    simp [eq]
 
-end MatchPartialShrink
+/- Helper lemma to avoid managing the greedy/lazy cases at the same time -/
+-- Actually, forgot about star difference...
+theorem matchPartialFree_or_comm {q r : Regex α} (mpf : [/⟨q⟩ | ⟨r⟩/].MatchPartialFree)
+    : [/⟨r⟩ | ⟨q⟩/].MatchPartialFree := by
+  rw [MatchPartialFree]
+  simp only [or_terminates_comm (q := r), mem_matchPartial_or_comm (q := r)]
+  exact mpf
+
+theorem matchPartialFree_star_greedy {r : Regex α} (rf : r.MatchPartialFree)
+    : [/⟨r⟩*/].MatchPartialFree := by
+  intro w s
+  by_cases! sle : s ≤ w.length
+  · induction s, sle using decreasingStrongRec with | ind s sle ind =>
+      simp only [matchPartial_star]
+      simp only [matchPartial_or, matchPartial_filterEmpty, ge_iff_le, eq_iff_iff, iff_true,
+        matchPartial_concat, Bool.false_eq_true, iff_false, not_le, matchPartial_empty,
+        List.mem_append, List.mem_filter, decide_eq_true_eq, List.mem_flatten,
+        List.mem_pmap, Prod.exists, ↓existsAndEq, true_and, List.mem_cons, List.not_mem_nil,
+        or_false, Prod.mk.injEq, Prod.forall]
+      intro cap term s'' cap'' mem wa wb cap₁ term₁
+      rcases mem with (mem | ⟨s', cap', mem, mem'⟩) | eq
+      · have ⟨cap₁', mem₁⟩ := rf _ _ _ _ _ mem.1 wa wb cap₁ (star_terminates.mp term₁).1
+        refine ⟨_, Or.inl (Or.inl ⟨mem₁, ?_⟩)⟩
+        have eq := le_antisymm mem.2 (monotone _ _ _ _ _ mem.1)
+        simp [eq]
+      · have s'le := endInBounds _ _ sle _ _ _ mem.1
+        specialize rf _ _ _ _ _ mem.1 wa (w.extract s' s'' ++ wb) cap₁
+        have rm := monotone _ _ _ _ _ mem.1
+        have rm' := monotone _ _ _ _ _ mem'
+        rw [List.extract_append_extract_assoc_right _ rm rm'] at rf
+        have ⟨cap₁', mem₁⟩ := rf (star_terminates.mp term₁).1
+        specialize ind s' s'le mem.2 _ _ _ mem' (wa ++ w.extract s s') wb cap₁'
+        rw [List.extract_append_extract_assoc_left _ rm rm'] at ind
+        have term₁ := (star_terminates.mp term₁).2 _ mem₁ (by
+          (suffices s < s' ∧ s < w.length by simpa); exact ⟨mem.2, trans mem.2 s'le⟩)
+        have ⟨cap₁'', mem₁'⟩ := ind term₁
+        rw [List.append_assoc _ (w.extract s s'), List.extract_append_extract _ rm rm'] at mem₁'
+        refine ⟨cap₁'', Or.inl (Or.inr ⟨_, _, ⟨mem₁, ?_⟩, mem₁'⟩)⟩
+        suffices s < s' ∧ s < w.length by simpa
+        exact ⟨mem.2, trans mem.2 s'le⟩
+      · refine ⟨cap₁, Or.inr ?_⟩
+        simp [eq]
+  · intro cap term mat mem wa wb cap₁ term₁
+    have bound := matchPartial_outOfBounds_eq (le_of_lt sle) mem
+    use cap₁
+    simp [bound, matchPartial_star, matchPartial_or, matchPartial_empty]
+
+theorem matchPartialFree_star_greedy_iff_lazy {r : Regex α}
+    : [/⟨r⟩*/].MatchPartialFree ↔ [/⟨r⟩*?/].MatchPartialFree := by
+  simp only [MatchPartialFree, star_terminates', matchPartial_star,
+    or_terminates_comm (q := [//]), mem_matchPartial_or_comm (q := [//])]
+  simp only [or_terminates, matchPartial_or, concat_terminates, matchPartial_concat,
+    star_terminates_greedy_iff_lazy, matchPartial_empty]
+  simp only [List.mem_append, List.mem_flatten, List.mem_pmap, ↓existsAndEq,
+    mem_matchPartial_star_greedy_iff_lazy]
+
+theorem matchPartialFree_star {t : StarType} {r : Regex α} (rf : r.MatchPartialFree)
+    : [/⟨r⟩*‹t›/].MatchPartialFree := by
+  cases t with
+  | greedy => exact matchPartialFree_star_greedy rf
+  | lazy => exact matchPartialFree_star_greedy_iff_lazy.mp (matchPartialFree_star_greedy rf)
+
+end MatchPartialFree
 
 def sndErasing {α β γ : Type*} (f : α × β → γ) := ∀ a b₁ b₂, f (a, b₁) = f (a, b₂)
 
 /-- Captures are irrelevant to the internal behavior of `matchPartial` in
 regular regexes. -/
 theorem limitRegular_matchPartial_eraseCaptures (rlim : classRegular r)
-    (w : List α) (s : Pos w)
+    (w : List α) (s : ℕ)
     : ∀ {β : Type*} (f : _ → β), sndErasing f → ∀ c₁ c₂,
       (r.matchPartial w s c₁).map f =
       (r.matchPartial w s c₂).map f := by
@@ -145,9 +188,9 @@ theorem limitRegular_matchPartial_eraseCaptures (rlim : classRegular r)
     simp only [matchPartial, List.pure_def, List.bind_eq_flatMap]
     simp only [List.map_flatMap, List.map_cons, List.map_nil]
     intro β f sf c₁ c₂
-    have pur (a : PosFrom s × Captures w)
-        : (fun a_1 : PosFrom a.1.pos × Captures w ↦ [f (a.1.widen a_1.1, a_1.2)]) =
-          pure ∘ (fun a_1 : PosFrom a.1.pos × Captures w ↦ f (a.1.widen a_1.1, a_1.2)) := by
+    have pur (a : PosFrom s × Captures)
+        : (fun a_1 : PosFrom a.1.pos × Captures ↦ [f (a.1.widen a_1.1, a_1.2)]) =
+          pure ∘ (fun a_1 : PosFrom a.1.pos × Captures ↦ f (a.1.widen a_1.1, a_1.2)) := by
       simp [Function.comp_def, List.pure_def]
     simp only [pur, List.flatMap_pure_eq_map]
     simp only [List.flatMap]
@@ -190,7 +233,7 @@ theorem limitRegular_matchPartial_eraseCaptures (rlim : classRegular r)
 and `star` behave nicely -/
 theorem limitRegular_isMatch_concat_star (rlim : classRegular r) (w : List α)
     : match r with
-      | concat p q => isMatch r w ↔ ∃ s : Pos w,
+      | concat p q => isMatch r w ↔ ∃ s : ℕ,
           isMatch p (w.take s.val) ∧ isMatch q (w.drop s.val)
       | star t q => isMatch r w ↔ (hw : w ≠ []) →
           ∃ s : PosFrom (Pos.succOfLt (List.length_pos_of_ne_nil hw)),
